src/LeanEVM/State.lean
@@ -1,0 +1,61 @@
+import LeanEVM.Util
+
+/- =============================================================== -/
+/- Bytecodes -/
+/- =============================================================== -/
+
+inductive Bytecode where
+| STOP
+| ADD
+| PUSH(n:u256)
+| POP
+| DUP
+
+/- =============================================================== -/
+/- Stack -/
+/- =============================================================== -/
+def EvmStack := List u256
+
+-- Pop an item of the EVM stack
+@[simp] def EvmStack.pop (st:EvmStack)(_:st.length > 0) : EvmStack :=
+  match st with
+  | _::t => t
+
+-- Push an item onto the EVM stack
+@[simp] def EvmStack.push (st:EvmStack)(n:u256) : EvmStack :=
+  n::st
+
+-- Peek an item on the EVM stack
+@[simp] def EvmStack.peek (st:EvmStack)(i:Fin st.length) : u256 :=
+  st.get i
+
+/- =============================================================== -/
+/- Ethereum Virtual Machine -/
+/- =============================================================== -/
+
+structure Evm where
+  stack: EvmStack
+
+@[simp] def Evm.pop (evm:Evm)(r:evm.stack.length > 0) : Evm :=
+  {stack:=evm.stack.pop r}
+
+@[simp] def Evm.push (evm:Evm)(n:u256) : Evm :=
+  {stack:=evm.stack.push n}
+
+@[simp] def Evm.peek (evm:Evm)(n:Nat)(r:n < evm.stack.length) : u256 :=
+  evm.stack.peek { val:= n, isLt := r}
+
+def EmptyEvm : Evm := {stack:=[]}
+
+/- =============================================================== -/
+/- Execution -/
+/- =============================================================== -/
+inductive Exception where
+| Revert
+| StackUnderflow
+| StackOverflow
+
+inductive Outcome where
+| Ok(evm: Evm)
+| Done (gas: Nat)(data: Array u8)
+| Error (err: Exception)
